% Equation 1
\begin{dmath}
{\hat{x}_{t}}={\hat{x}_{t+1}}-\frac{1}{{\sigma}}\, \left({\hat{i}_{t}}-{\hat{\pi}_{t+1}}\right)+{\hat{u}_{t}}
\end{dmath}
% Equation 2
\begin{dmath}
{\hat{\pi}_{t}}={\hat{\pi}_{t+1}}\, {\beta}+{\hat{x}_{t}}\, {\kappa}+{\hat{\varepsilon^{\pi}}_{t}}
\end{dmath}
% Equation 3
\begin{dmath}
{\hat{i}_{t}}={\hat{\pi}_{t}}\, {\rho_{\pi}}+{\hat{\nu}_{t}}
\end{dmath}
% Equation 4
\begin{dmath}
{\hat{u}_{t}}={\rho_u}\, {\hat{u}_{t-1}}+{\hat{\varepsilon^{u}}_{t}}
\end{dmath}
% Equation 5
\begin{dmath}
{\hat{\nu}_{t}}={\rho_{\nu}}\, {\hat{\nu}_{t-1}}+{\hat{\varepsilon^{\nu}}_{t}}
\end{dmath}
